wip: curve25519

specs/Spec.Curve25519.fst
@@ -2,37 +2,61 @@ module Spec.Curve25519
 
 open FStar.Mul
 open Lib.IntTypes
-open Lib.RawIntTypes
 open Lib.Sequence
 open Lib.ByteSequence
-open Lib.NatMod
-open Lib.LoopCombinators
+
 open Spec.Curve25519.Lemmas
 
-
-#reset-options "--max_fuel 0 --z3rlimit 20"
-
 (* Field types and parameters *)
-let prime = pow2 255 - 19
+let prime : pos = pow2 255 - 19
 
-unfold type elem = nat_mod prime
-let to_elem x = x `modulo` prime
-let from_elem (x:elem) = nat_mod_v x
-let zero : elem = to_elem 0
-let one  : elem = to_elem 1
+type elem = x:nat{x < prime}
+let zero : elem = 0
+let one  : elem = 1
+
+let fadd (x:elem) (y:elem) : elem = (x + y) % prime
+let fsub (x:elem) (y:elem) : elem = (x - y) % prime
+let fmul (x:elem) (y:elem) : elem = (x * y) % prime
+
+let ( +% ) = fadd
+let ( -% ) = fsub
+let ( *% ) = fmul
+
+val pow: a:elem -> b:nat -> res:elem
+let rec pow a b =
+  if b = 0 then 1
+  else fmul a (pow a (b - 1))
+
+val fpow: a:elem -> b:pos -> Tot (res:elem) (decreases b)
+let rec fpow a b =
+  if b = 1 then a
+  else
+    if b % 2 = 0 then fpow (a *% a) (b / 2)
+    else a *% (fpow (a *% a) (b / 2))
+
+let ( **% ) = fpow
 
 (* Type aliases *)
 type scalar = lbytes 32
 type serialized_point = lbytes 32
-noeq type proj_point = | Proj: x:elem -> z:elem -> proj_point
+type proj_point = elem & elem
+
+let ith_bit (k:scalar) (i:nat{i < 256}) : uint8 =
+  let q = i / 8 in let r = size (i % 8) in
+  (k.[q] >>. r) &. u8 1
 
 let decodePoint (u:serialized_point) =
-  to_elem (nat_from_bytes_le u % pow2 255)
+  (nat_from_bytes_le u % pow2 255) % prime
+
+let encodePoint (p:proj_point) : Tot serialized_point =
+  let x, z = p in
+  let p = x *% (z **% (prime - 2)) in
+  nat_to_bytes_le 32 p
 
 let add_and_double q nq nqp1 =
-  let x_1, z_1 = q.x, q.z in
-  let x_2, z_2 = nq.x, nq.z in
-  let x_3, z_3 = nqp1.x, nqp1.z in
+  let x_1, z_1 = q in
+  let x_2, z_2 = nq in
+  let x_3, z_3 = nqp1 in
   let a  = x_2 +% z_2 in
   let b  = x_2 -% z_2 in
   let c = x_3 +% z_3 in
@@ -41,70 +65,74 @@ let add_and_double q nq nqp1 =
   let cb = c *% b in
   let x_3 = da +% cb in
   let z_3 = da -% cb in
-  let aa = a  **% 2 in
-  let bb = b  **% 2 in
-  let x_3 = x_3  **% 2 in
-  let z_3 = z_3  **% 2 in
+  let aa = a **% 2 in
+  let bb = b **% 2 in
+  let x_3 = x_3 **% 2 in
+  let z_3 = z_3 **% 2 in
   let e = aa -% bb in
   let e121665 = e *% 121665 in
-  let aa_e121665 = e121665 +% aa in 
+  let aa_e121665 = e121665 +% aa in
   let x_2 = aa *% bb in
   let z_2 = e *% aa_e121665 in
   let z_3 = z_3 *% x_1 in
-  Proj x_2 z_2, Proj x_3 z_3
+  (x_2, z_2), (x_3, z_3)
 
 let double nq =
-  let x_2, z_2 = nq.x, nq.z in
+  let x_2, z_2 = nq in
   let a  = x_2 +% z_2 in
   let b  = x_2 -% z_2 in
-  let aa = a  **% 2 in
-  let bb = b  **% 2 in
+  let aa = a **% 2 in
+  let bb = b **% 2 in
   let e = aa -% bb in
   let e121665 = e *% 121665 in
-  let aa_e121665 = e121665 +% aa in 
+  let aa_e121665 = e121665 +% aa in
   let x_2 = aa *% bb in
   let z_2 = e *% aa_e121665 in
-  Proj x_2 z_2
+  x_2, z_2
 
-
-let ith_bit (k:scalar) (i:nat{i < 256}) : uint8 =
-  let (&.) = logand #U8 in
-  let q = i / 8 in let r = size (i % 8) in
-  (k.[q] >>. r) &. u8 1
-
-let ladder_step (q:proj_point) (bit:uint8) (nq,nqp1) =
+let ladder_step (q:proj_point) (bit:uint8) (nq, nqp1) =
+  let open Lib.RawIntTypes in
   if uint_to_nat bit = 1 then (
      let nqp1, nq = add_and_double q nqp1 nq in
      nq, nqp1)
-  else add_and_double q nq nqp1 
-  
+  else add_and_double q nq nqp1
+
 let montgomery_ladder (init:elem) (k:scalar) : Tot proj_point =
-  let q = Proj init one in
-  let nq = Proj one zero in
-  let nqp1 = Proj init one in
+  let q = (init, one) in
+  let nq = (one, zero) in
+  let nqp1 = (init, one) in
   // bit 255 is 0 and bit 254 is 1
   let nqp1,nq = add_and_double q nqp1 nq in
   // bits 253-3 depend on scalar
-  let nq,nqp1 = repeati 251
-    (fun i -> ladder_step q (ith_bit k (253-i))) (nq,nqp1) in
-  // bits 2-0 are 0 
+  let nq,nqp1 = Lib.LoopCombinators.repeati 251
+    (fun i -> ladder_step q (ith_bit k (253-i))) (nq, nqp1) in
+  // bits 2-0 are 0
   let nq = double nq in
   let nq = double nq in
   let nq = double nq in
-  nq  
+  nq
 
-
-let encodePoint (p:proj_point) : Tot serialized_point =
-  let p = p.x *% (p.z   **%  (prime - 2)) in
-  nat_to_bytes_le 32 (from_elem p)
 
 let scalarmult (k:scalar) (u:serialized_point) : Tot serialized_point =
   let u = decodePoint u in
   let res = montgomery_ladder u k in
   encodePoint res
 
-val secret_to_public: lbytes 32 -> Tot (lbytes 32)
+inline_for_extraction
+let basepoint_list : x:list byte_t{List.Tot.length x == 32} =
+  [@inline_let]
+  let l =
+    [9uy; 0uy; 0uy; 0uy; 0uy; 0uy; 0uy; 0uy;
+    0uy; 0uy; 0uy; 0uy; 0uy; 0uy; 0uy; 0uy;
+    0uy; 0uy; 0uy; 0uy; 0uy; 0uy; 0uy; 0uy;
+    0uy; 0uy; 0uy; 0uy; 0uy; 0uy; 0uy; 0uy] in
+  assert_norm (List.Tot.length l == 32);
+  l
+
+let basepoint_lseq : Lib.Sequence.lseq byte_t 32 =
+  Lib.Sequence.of_list basepoint_list
+
+val secret_to_public: lbytes 32 -> lbytes 32
 let secret_to_public kpriv =
-  let basepoint_zeros = create 32 (u8 0) in
-  let basepoint = upd basepoint_zeros (32 - 1) (u8 0x09) in
+  let basepoint = map secret basepoint_lseq in
   scalarmult kpriv basepoint
